x86/Stacklayout.v
@@ -31,39 +31,24 @@ Local Open Scope sep_scope.
 
 Definition fe_ofs_arg := 0.
 
-(* Definition make_env (b: bounds) : frame_env := *)
-(*   let w := if Archi.ptr64 then 8 else 4 in *)
-(*   let ocs := align (4 * b.(bound_outgoing)) w in  (* back link *) *)
-(*   (* let ocs := olink + w in                           (* callee-saves *) *) *)
-(*   let ol :=  align (size_callee_save_area b ocs) 8 in (* locals *) *)
-(*   let ostkdata := align (ol + 4 * b.(bound_local)) 8 in (* stack data *) *)
-(*   let oretaddr := align (ostkdata + b.(bound_stack_data)) w in (* return address *) *)
-(*   let sz := oretaddr + w in (* total size *) *)
-(*   {| fe_size := sz; *)
-(*      (* fe_ofs_link := olink; *) *)
-(*      fe_ofs_retaddr := oretaddr; *)
-(*      fe_ofs_local := ol; *)
-(*      fe_ofs_callee_save := ocs; *)
-(*      fe_stack_data := ostkdata; *)
-(*      fe_used_callee_save := b.(used_callee_save) |}. *)
-
 Definition make_env (b: bounds) : frame_env :=
   let w := if Archi.ptr64 then 8 else 4 in
-  let ocs := align (4 * b.(bound_outgoing)) w in  (* back link *)
-  (* let ocs := olink + w in                           (* callee-saves *) *)
+(*  let olink := align (4 * b.(bound_outgoing)) w in  (* back link *) *)
+  let ocs := align (4 * b.(bound_outgoing)) w (*SACC:comments this*)(*+ w*) in  (* callee-saves *)
   let ol :=  align (size_callee_save_area b ocs) 8 in (* locals *)
   let ostkdata := align (ol + 4 * b.(bound_local)) 8 in (* stack data *)
   let preretaddr := align (ostkdata + b.(bound_stack_data)) w in
   let sz := align (preretaddr + w) 8 in (* total size *)
   let oretaddr := sz - w in (* return address *)
   {| fe_size := sz;
-     (* fe_ofs_link := olink; *)
+(*SACC: comments this*)(*fe_ofs_link := olink;*)
      fe_ofs_retaddr := oretaddr;
      fe_ofs_local := ol;
      fe_ofs_callee_save := ocs;
      fe_stack_data := ostkdata;
      fe_used_callee_save := b.(used_callee_save) |}.
 
+(*SACC:*)
 Lemma retaddr_le: forall preretaddr w,
   preretaddr <= (align (preretaddr + w) 8) - w.
 Proof.
@@ -73,72 +58,148 @@ Proof.
   omega.
 Qed.
 
-Section WITHMEM.
-  Context `{memory_model_prf: Mem.MemoryModel}.
-  Lemma frame_env_separated:
-    forall b sp (m: mem) P,
-      let fe := make_env b in
-      m |= range sp 0 (fe_stack_data fe) ** range sp (fe_stack_data fe + bound_stack_data b) (fe_size fe) ** P ->
-      m |= range sp (fe_ofs_local fe) (fe_ofs_local fe + 4 * bound_local b)
-        ** range sp fe_ofs_arg (fe_ofs_arg + 4 * bound_outgoing b)
-        (* ** range sp (fe_ofs_link fe) (fe_ofs_link fe + size_chunk Mptr) *)
-        ** range sp (fe_ofs_retaddr fe) (fe_ofs_retaddr fe + size_chunk Mptr)
-        ** range sp (fe_ofs_callee_save fe) (size_callee_save_area b (fe_ofs_callee_save fe))
-        ** P.
-  Proof.
-    Local Opaque Z.add Z.mul sepconj range.
-    intros; simpl.
-    set (w := if Archi.ptr64 then 8 else 4).
-    set (ocs := align (4 * b.(bound_outgoing)) w).
-    (* set (ocs := olink + w). *)
-    set (ol :=  align (size_callee_save_area b ocs) 8).
-    set (ostkdata := align (ol + 4 * b.(bound_local)) 8).
-    set (preretaddr := align (ostkdata + b.(bound_stack_data)) w).
-    set (sz := align (preretaddr + w) 8).
-    set (oretaddr := sz - w).
-    assert (preretaddr <= oretaddr) as RET by apply retaddr_le.
-    replace (size_chunk Mptr) with w by (rewrite size_chunk_Mptr; auto).
-    assert (0 < w) by (unfold w; destruct Archi.ptr64; omega).
-    generalize b.(bound_local_pos) b.(bound_outgoing_pos) b.(bound_stack_data_pos); intros.
-    assert (0 <= 4 * b.(bound_outgoing)) by omega.
-    assert (4 * b.(bound_outgoing) <= ocs) by (apply align_le; omega).
-    (* assert (olink + w <= ocs) by (unfold ocs; omega). *)
-    assert (ocs <= size_callee_save_area b ocs) by (apply size_callee_save_area_incr).
-    assert (size_callee_save_area b ocs <= ol) by (apply align_le; omega).
-    assert (ol + 4 * b.(bound_local) <= ostkdata) by (apply align_le; omega).
-    assert (ostkdata + bound_stack_data b <= oretaddr).
-    { 
-      apply Z.le_trans with (align (ostkdata + bound_stack_data b) w).
-      apply align_le. omega.
-      subst preretaddr. omega.
-    }
-    (* Reorder as: *)
-  (*    outgoing *)
-  (*    callee-save *)
-  (*    local *)
-  (*    retaddr *)
-    rewrite sep_swap12.
-    rewrite sep_swap23.
-    rewrite sep_swap34.
-    rewrite sep_swap23.
-    rewrite sep_swap34.
-    (* Apply range_split and range_split2 repeatedly *)
-    unfold fe_ofs_arg.
-    apply range_split_2. fold ocs. omega. omega.
-    apply range_split_2. fold ol. omega. omega.
-    apply range_drop_right with ostkdata. omega.
-    rewrite sep_swap.
-    apply range_drop_left with (ostkdata + bound_stack_data b). omega.
-    rewrite sep_swap.
-    assert (oretaddr + w = fe_size fe) as SZEQ. 
-    { 
-      subst fe. subst w ocs ol ostkdata preretaddr oretaddr sz. 
-      unfold make_env. simpl. omega.
-    }
-    rewrite SZEQ.
-    exact H.
-  Qed.
+Lemma frame_env_separated:
+  forall b sp m P,
+  let fe := make_env b in
+  m |= range sp 0 (fe_stack_data fe) ** range sp (fe_stack_data fe + bound_stack_data b) (fe_size fe) ** P ->
+  m |= range sp (fe_ofs_local fe) (fe_ofs_local fe + 4 * bound_local b)
+       ** range sp fe_ofs_arg (fe_ofs_arg + 4 * bound_outgoing b)
+      (*SACC:comments this*)(* ** range sp (fe_ofs_link fe) (fe_ofs_link fe + size_chunk Mptr) *)
+       ** range sp (fe_ofs_retaddr fe) (fe_ofs_retaddr fe + size_chunk Mptr)
+       ** range sp (fe_ofs_callee_save fe) (size_callee_save_area b (fe_ofs_callee_save fe))
+       ** P.
+Proof.
+Local Opaque Z.add Z.mul sepconj range.
+  intros; simpl.
+  set (w := if Archi.ptr64 then 8 else 4).
+  (*SACC: comments this*)(*set (olink := align (4 * b.(bound_outgoing)) w).*)
+  (*SACC: comments this*)(*set (ocs := olink + w).*)
+  set (ocs := align (4 * b.(bound_outgoing)) w).
+  set (ol :=  align (size_callee_save_area b ocs) 8).
+  set (ostkdata := align (ol + 4 * b.(bound_local)) 8).
+  (*SACC:*)set (preretaddr := align (ostkdata + b.(bound_stack_data)) w).
+  (*SACC:*)set (sz := align (preretaddr + w) 8).
+  (*SACC:comments this*)(*set (oretaddr := align (ostkdata + b.(bound_stack_data)) w).*)
+  (*SACC:*)set (oretaddr := sz - w).
+  replace (size_chunk Mptr) with w by (rewrite size_chunk_Mptr; auto).
+  assert (0 < w) by (unfold w; destruct Archi.ptr64; omega).
+  generalize b.(bound_local_pos) b.(bound_outgoing_pos) b.(bound_stack_data_pos); intros.
+  assert (0 <= 4 * b.(bound_outgoing)) by omega.
+  assert (4 * b.(bound_outgoing) <= (*SACC:*)(*olink*)ocs) by (apply align_le; omega).
+  (*SACC:comments this*)(*assert (olink + w <= ocs) by (unfold ocs; omega).*)
+  assert (preretaddr <= oretaddr) as RET by apply retaddr_le.
+  assert (ocs <= size_callee_save_area b ocs) by (apply size_callee_save_area_incr). 
+  assert (size_callee_save_area b ocs <= ol) by (apply align_le; omega).
+  assert (ol + 4 * b.(bound_local) <= ostkdata) by (apply align_le; omega).
+  assert (ostkdata + bound_stack_data b <= oretaddr).
+  {
+    apply Z.le_trans with (align (ostkdata + bound_stack_data b) w).
+    apply align_le. omega.
+    subst preretaddr. omega.
+  }
+  (*SACC:*)assert (oretaddr + w = fe_size fe) as SZEQ. 
+  { 
+    subst fe. subst w ocs ol ostkdata preretaddr oretaddr sz. 
+    unfold make_env. simpl. omega.
+  }
+(* Reorder as:
+     outgoing
+     back link
+     callee-save
+     local
+     retaddr *)
+  rewrite sep_swap12.
+  rewrite sep_swap23.
+  rewrite sep_swap34.
+  rewrite sep_swap23.
+  rewrite sep_swap34.
+(* Apply range_split and range_split2 repeatedly *)
+  unfold fe_ofs_arg.
+  apply range_split_2. fold ocs. omega. omega. 
+  (*apply range_split. omega.*)
+  apply range_split_2. fold ol. omega. omega.
+  apply range_drop_right with ostkdata. omega.
+  rewrite sep_swap.
+  apply range_drop_left with (ostkdata + bound_stack_data b). omega.
+  rewrite sep_swap.
+  rewrite SZEQ. exact H.
+Qed.
 
+Lemma frame_env_range:
+  forall b,
+  let fe := make_env b in
+  0 <= fe_stack_data fe /\ fe_stack_data fe + bound_stack_data b <= fe_size fe.
+Proof.
+  intros; simpl.
+  set (w := if Archi.ptr64 then 8 else 4).
+  (*SACC:comments this*)(*set (olink := align (4 * b.(bound_outgoing)) w).*)
+  (*SACC:comments this*)(*set (ocs := olink + w).*)
+  (*SACC:*)set (ocs := align (4 * b.(bound_outgoing)) w).
+  set (ol :=  align (size_callee_save_area b ocs) 8).
+  set (ostkdata := align (ol + 4 * b.(bound_local)) 8).
+  (*SACC:*)set (preretaddr := align (ostkdata + b.(bound_stack_data)) w).
+  (*SACC:comments this*)(*set (oretaddr := align (ostkdata + b.(bound_stack_data)) w).*)
+  (*SACC:*)set (sz := align (preretaddr + w) 8).
+  (*SACC:*)set (oretaddr := sz - w).
+  assert (0 < w) by (unfold w; destruct Archi.ptr64; omega).
+  generalize b.(bound_local_pos) b.(bound_outgoing_pos) b.(bound_stack_data_pos); intros.
+  assert (0 <= 4 * b.(bound_outgoing)) by omega.
+  assert (4 * b.(bound_outgoing) <= (*SACC:*)(*olink*)ocs) by (apply align_le; omega).
+  (*SACC:*)(*assert (olink + w <= ocs) by (unfold ocs; omega).*)
+  assert (ocs <= size_callee_save_area b ocs) by (apply size_callee_save_area_incr). 
+  assert (size_callee_save_area b ocs <= ol) by (apply align_le; omega).
+  assert (ol + 4 * b.(bound_local) <= ostkdata) by (apply align_le; omega).
+  (*SACC:*)assert (preretaddr <= oretaddr) as RET by apply retaddr_le.
+  assert (ostkdata + bound_stack_data b <= oretaddr). 
+  {
+    apply Z.le_trans with (align (ostkdata + bound_stack_data b) w).
+    apply align_le. omega.
+    subst preretaddr. omega.
+  }
+  split. omega. subst oretaddr. omega. 
+Qed.
+
+Lemma frame_env_aligned:
+  forall b,
+  let fe := make_env b in
+     (8 | fe_ofs_arg)
+  /\ (8 | fe_ofs_local fe)
+  /\ (8 | fe_stack_data fe)
+(*  /\ (align_chunk Mptr | fe_ofs_link fe) *)
+  /\ (align_chunk Mptr | fe_ofs_retaddr fe).
+Proof.
+  intros; simpl.
+  set (w := if Archi.ptr64 then 8 else 4).
+  (*SACC: comments this*)
+  (*set (olink := align (4 * b.(bound_outgoing)) w).
+  set (ocs := olink + w).*)
+  (*SACC:*)set (ocs := align (4 * b.(bound_outgoing)) w).
+  set (ol :=  align (size_callee_save_area b ocs) 8).
+  set (ostkdata := align (ol + 4 * b.(bound_local)) 8).
+  (*SACC:*)set (preretaddr := align (ostkdata + b.(bound_stack_data)) w).
+  (*SACC:*)set (sz := align (preretaddr + w) 8).
+  (*SACC:comments this*)(*
+  set (oretaddr := align (ostkdata + b.(bound_stack_data)) w).*)
+  set (oretaddr := sz - w).
+  assert (0 < w) by (unfold w; destruct Archi.ptr64; omega).
+  assert (w_divides8: (w | 8)).
+  {
+    simpl. unfold w. destr. apply Z.divide_refl.
+    apply Zdivide_intro with 2. omega.
+  }
+  (*SACC:*)assert (preretaddr <= oretaddr) as RET by apply retaddr_le.
+  replace (align_chunk Mptr) with w by (rewrite align_chunk_Mptr; auto).
+  split. apply Zdivide_0.
+  split. apply align_divides; omega.
+  split. apply align_divides; omega.
+  subst oretaddr. apply Z.divide_sub_r. 
+  subst sz. apply Z.divide_trans with 8. apply w_divides8.
+  apply align_divides; omega.
+  apply Z.divide_refl.
+Qed.
+
+
+(*========================SACC:========================*)
 
 Lemma frame_env_separated':
   (* forall `{memory_model_prf: Mem.MemoryModel} *)
@@ -177,95 +238,6 @@ Local Transparent fe_stack_data.
 simpl. fold w. fold ocs. fold ol. fold ostkdata. omega.
 Qed.
 
-Lemma frame_env_range:
-  forall b,
-  let fe := make_env b in
-  0 <= fe_stack_data fe /\ fe_stack_data fe + bound_stack_data b <= fe_size fe.
-Proof.
-  intros; simpl.
-  set (w := if Archi.ptr64 then 8 else 4).
-  set (ocs := align (4 * b.(bound_outgoing)) w).
-  (* set (ocs := olink + w). *)
-  set (ol :=  align (size_callee_save_area b ocs) 8).
-  set (ostkdata := align (ol + 4 * b.(bound_local)) 8).
-  set (preretaddr := align (ostkdata + b.(bound_stack_data)) w).
-  set (sz := align (preretaddr + w) 8).
-  set (oretaddr := sz - w).
-  assert (preretaddr <= oretaddr) as RET by apply retaddr_le.
-  assert (0 < w) by (unfold w; destruct Archi.ptr64; omega).
-  generalize b.(bound_local_pos) b.(bound_outgoing_pos) b.(bound_stack_data_pos); intros.
-  assert (0 <= 4 * b.(bound_outgoing)) by omega.
-  assert (4 * b.(bound_outgoing) <= ocs) by (apply align_le; omega).
-  assert (ocs <= size_callee_save_area b ocs) by (apply size_callee_save_area_incr).
-  assert (size_callee_save_area b ocs <= ol) by (apply align_le; omega).
-  assert (ol + 4 * b.(bound_local) <= ostkdata) by (apply align_le; omega).
-  assert (ostkdata + bound_stack_data b <= oretaddr).
-  { 
-    apply Z.le_trans with (align (ostkdata + bound_stack_data b) w).
-    apply align_le. omega.
-    subst preretaddr. omega.
-  }
-  split. omega. subst oretaddr. omega.
-Qed.
-
-Lemma w_divides8 :
-  let w := if Archi.ptr64 then 8 else 4 in
-  (w | 8).
-Proof.
-  simpl. destr. apply Z.divide_refl.
-  apply Zdivide_intro with 2. omega.
-Qed.
-
-Lemma frame_env_aligned:
-  forall b,
-  let fe := make_env b in
-     (8 | fe_ofs_arg)
-  /\ (8 | fe_ofs_local fe)
-  /\ (8 | fe_stack_data fe)
-  (* /\ (align_chunk Mptr | fe_ofs_link fe) *)
-  /\ (align_chunk Mptr | fe_ofs_retaddr fe).
-Proof.
-  intros; simpl.
-  set (w := if Archi.ptr64 then 8 else 4).
-  set (ocs := align (4 * b.(bound_outgoing)) w).
-  set (ol :=  align (size_callee_save_area b ocs) 8).
-  set (ostkdata := align (ol + 4 * b.(bound_local)) 8).
-  set (preretaddr := align (ostkdata + b.(bound_stack_data)) w).
-  set (sz := align (preretaddr + w) 8).
-  set (oretaddr := sz - w).
-  assert (preretaddr <= oretaddr) as RET by apply retaddr_le.
-  assert (0 < w) by (unfold w; destruct Archi.ptr64; omega).
-  replace (align_chunk Mptr) with w by (rewrite align_chunk_Mptr; auto).
-  split. apply Zdivide_0.
-  split. apply align_divides; omega.
-  split. apply align_divides; omega.
-  subst oretaddr. apply Z.divide_sub_r. 
-  subst sz. apply Z.divide_trans with 8. apply w_divides8.
-  apply align_divides; omega.
-  apply Z.divide_refl.
-Qed.
-
-Lemma le_add_pos:
-  forall a b,
-    0 <= b ->
-    a <= a + b.
-Proof.
-  intros; omega.
-Qed.
-
-Lemma lt_add_pos:
-  forall a b,
-    0 < b ->
-    a < a + b.
-Proof.
-  intros; omega.
-Qed.
-
-
-(* fe_ofs_link fe_ofs_retaddr fe_size fe_ofs_local  fe_ofs_arg *)
-(*        fe_ofs_callee_save  fe_stack_data. *)
-Opaque bound_local bound_outgoing  size_callee_save_area bound_stack_data.
-
 Lemma zero_lt_align8 : forall x,
   0 < x -> 0 < align x 8.
 Proof.
@@ -292,266 +264,3 @@ Proof.
   generalize (bound_outgoing_pos b); omega.
 Qed.
 
-Lemma zero_le_align8 : forall x,
-  0 <= x -> 0 <= align x 8.
-Proof.
-  intros.
-  eapply Z.le_trans. 
-  Focus 2. apply align_le. omega.
-  auto.
-Qed.
-
-(* Lemma zero_le_alignw : forall x, *)
-(*   0 <= x -> 0 <= align x (if Archi.ptr64 then 8 else 4). *)
-(* Proof. *)
-(*   intros. *)
-(*   eapply Z.le_trans.  *)
-(*   Focus 2. apply align_le. destr; omega. *)
-(*   auto. *)
-(* Qed. *)
-
-
-Program Definition frame_of_frame_env (b: bounds) : frame_info :=
-  let fe := make_env b in
-  {|
-    frame_size := fe_size fe;
-    frame_perm := fun o =>
-                    if zle (fe_stack_data fe) o && zlt o (fe_stack_data fe + bound_stack_data b)
-                    then Public
-                    else Private
-  |}.
-Next Obligation.
-  apply zero_le_align8. etransitivity. 2: apply le_add_pos. 2: destr; omega.
-  etransitivity. 2: apply align_le. 2: destr; omega.
-  etransitivity. 2: apply le_add_pos. 2: generalize (bound_stack_data_pos b); omega.
-  etransitivity. 2: apply align_le. 2: omega.
-  etransitivity. 2: apply le_add_pos. 2: generalize (bound_local_pos b); omega.
-  etransitivity. 2: apply align_le. 2: omega.
-  etransitivity. 2: apply size_callee_save_area_incr.
-  etransitivity. 2: apply align_le. 2: destr; omega.
-  generalize (bound_outgoing_pos b); omega.
-Qed.
-
-Lemma stkdata_retaddr_sep:
-  forall b,
-    let fe := make_env b in
-    forall o,
-      fe_stack_data fe <= o < fe_stack_data fe + bound_stack_data b ->
-      fe_ofs_retaddr fe <= o < fe_ofs_retaddr fe + size_chunk Mptr ->
-      False.
-Proof.
-  clear. intros b fe.
-  generalize (frame_env_separated' b).
-  intros.
-  destruct H. destruct H2. destruct H3. destruct H4. destruct H5.
-  set (w := if Archi.ptr64 then 8 else 4) in *.
-  set (ocs := align (4 * b.(bound_outgoing)) w) in *.
-  set (ol :=  align (size_callee_save_area b ocs) 8) in *.
-  set (ostkdata := align (ol + 4 * b.(bound_local)) 8) in *.
-  set (preretaddr := align (ostkdata + b.(bound_stack_data)) w) in *.
-  set (sz := align (preretaddr + w) 8) in *.
-  set (oretaddr := sz - w) in *.
-  assert (preretaddr <= oretaddr) as RET by apply retaddr_le.
-  subst w ocs ol ostkdata preretaddr sz oretaddr. simpl in *. omega.
-Qed.
-
-
-Lemma arg_retaddr_sep:
-  forall b,
-    let fe := make_env b in
-    forall o,
-      fe_ofs_arg <= o < fe_ofs_arg + 4 * bound_outgoing b ->
-      fe_ofs_retaddr fe <= o < fe_ofs_retaddr fe + size_chunk Mptr ->
-      False.
-Proof.
-  clear. intros b fe.
-  generalize (frame_env_separated' b).
-  intros.
-  destruct H. destruct H2. destruct H3. destruct H4. destruct H5.
-  set (w := if Archi.ptr64 then 8 else 4) in *.
-  set (ocs := align (4 * b.(bound_outgoing)) w) in *.
-  set (ol :=  align (size_callee_save_area b ocs) 8) in *.
-  set (ostkdata := align (ol + 4 * b.(bound_local)) 8) in *.
-  set (preretaddr := align (ostkdata + b.(bound_stack_data)) w) in *.
-  set (sz := align (preretaddr + w) 8) in *.
-  set (oretaddr := sz - w) in *.
-  assert (preretaddr <= oretaddr) as RET by apply retaddr_le.
-  cut (fe_ofs_arg + 4 * bound_outgoing b <= oretaddr). 
-  subst w ocs ol ostkdata preretaddr sz oretaddr. simpl in *. omega.
-  eapply Z.le_trans. 2: eauto. 
-  unfold preretaddr. 
-  unfold fe_ofs_arg. rewrite Z.add_0_l.
-  eapply Z.le_trans with ocs. unfold ocs. apply align_le. unfold w; destr; omega.
-  eapply Z.le_trans. exact H2. 
-  apply Z.le_trans with ol. unfold ol. apply align_le; omega.
-  eapply Z.le_trans. apply le_add_pos with (b:= 4* bound_local b).
-  generalize (bound_local_pos b); omega.
-  apply Z.le_trans with ostkdata; auto.
-  eapply Z.le_trans. apply le_add_pos with (b:= bound_stack_data b).
-  generalize (bound_stack_data_pos b); omega.
-  apply align_le. unfold w; destr; omega.
-Qed.
-
-Lemma arg_local_sep:
-  forall b,
-    let fe := make_env b in
-    forall o,
-      fe_ofs_arg <= o < fe_ofs_arg + 4 * bound_outgoing b ->
-      fe_ofs_local fe <= o < fe_ofs_local fe + 4 * bound_local b ->
-      False.
-Proof.
-  clear. intros b fe.
-  generalize (frame_env_separated' b).
-  simpl. intuition.
-  cut (o<o). omega.
-  eapply Z.lt_le_trans. apply H8.
-  etransitivity. 2: apply H4.
-  etransitivity. 2: apply align_le; try (omega).
-  etransitivity. 2: apply size_callee_save_area_incr.
-  change fe_ofs_arg with 0.
-  rewrite Z.add_0_l.
-  apply align_le. destr; omega.
-Qed.
-
-Lemma arg_callee_save_sep:
-  forall b,
-    let fe := make_env b in
-    forall o,
-      fe_ofs_arg <= o < fe_ofs_arg + 4 * bound_outgoing b ->
-      fe_ofs_callee_save fe <= o < size_callee_save_area b (fe_ofs_callee_save fe) ->
-      False.
-Proof.
-  clear. intros b fe.
-  generalize (frame_env_separated' b).
-  simpl. intuition.
-  cut (o<o). omega.
-  eapply Z.lt_le_trans. apply H8.
-  etransitivity. 2: apply H4.
-  change fe_ofs_arg with 0.
-  rewrite Z.add_0_l.
-  apply align_le. destr; omega.
-Qed.
-
-Lemma local_retaddr_sep:
-  forall b,
-    let fe := make_env b in
-    forall o,
-      fe_ofs_local fe <= o < fe_ofs_local fe + 4 * bound_local b ->
-      fe_ofs_retaddr fe <= o < fe_ofs_retaddr fe + size_chunk Mptr ->
-      False.
-Proof.
-  clear. intros b fe.
-  generalize (frame_env_separated' b).
-  intros.
-  destruct H. destruct H2. destruct H3. destruct H4. destruct H5.
-  set (w := if Archi.ptr64 then 8 else 4) in *.
-  set (ocs := align (4 * b.(bound_outgoing)) w) in *.
-  set (ol :=  align (size_callee_save_area b ocs) 8) in *.
-  set (ostkdata := align (ol + 4 * b.(bound_local)) 8) in *.
-  set (preretaddr := align (ostkdata + b.(bound_stack_data)) w) in *.
-  set (sz := align (preretaddr + w) 8) in *.
-  set (oretaddr := sz - w) in *.
-  assert (preretaddr <= oretaddr) as RET by apply retaddr_le.
-  cut (ol + 4 * bound_local b <= oretaddr). 
-  subst w ocs ol ostkdata preretaddr sz oretaddr. simpl in *. omega.
-  eapply Z.le_trans. 2: exact RET.
-  unfold preretaddr.
-  eapply Z.le_trans. eauto.
-  eapply Z.le_trans. apply le_add_pos with (b:= bound_stack_data b).
-  generalize (bound_stack_data_pos b); omega.
-  apply align_le. unfold w; destr; omega.
-Qed.
-
-Lemma local_callee_save_sep:
-  forall b,
-    let fe := make_env b in
-    forall o,
-      fe_ofs_local fe <= o < fe_ofs_local fe + 4 * bound_local b ->
-      fe_ofs_callee_save fe <= o < size_callee_save_area b (fe_ofs_callee_save fe) ->
-      False.
-Proof.
-  clear. intros b fe.
-  generalize (frame_env_separated' b).
-  simpl. intuition.
-Qed.
-
-Lemma stkdata_callee_save_sep:
-  forall b,
-    let fe := make_env b in
-    forall o,
-      fe_stack_data fe <= o < fe_stack_data fe + bound_stack_data b ->
-      fe_ofs_callee_save fe <= o < size_callee_save_area b (fe_ofs_callee_save fe) ->
-      False.
-Proof.
-  clear. intros b fe.
-  generalize (frame_env_separated' b).
-  simpl. intuition.
-  cut (o < o). omega.
-  eapply Z.lt_le_trans.
-  apply H9. etransitivity.
-  2: apply H7.
-  etransitivity. 2: apply align_le ; try omega.
-  etransitivity. 2: apply le_add_pos; [ generalize (bound_local_pos b); omega].
-  apply align_le. omega.
-Qed.
-
-Lemma local_arg_sep:
-  forall b,
-    let fe := make_env b in
-    forall o,
-      fe_ofs_local fe <= o < fe_ofs_local fe + 4 * bound_local b ->
-      fe_ofs_arg <= o < fe_ofs_arg + 4 * bound_outgoing b ->
-      False.
-Proof.
-  clear. intros b fe.
-  generalize (frame_env_separated' b).
-  simpl. intuition.
-    cut (o < o). omega.
-  eapply Z.lt_le_trans.
-  apply H9. etransitivity.
-  2: apply H7.
-  etransitivity. 2: apply align_le ; try omega.
-  etransitivity. 2: apply size_callee_save_area_incr.
-  change fe_ofs_arg with 0.
-  rewrite Z.add_0_l.
-  apply align_le. destr; omega.
-Qed.
-
-Lemma stkdata_arg_sep:
-  forall b,
-    let fe := make_env b in
-    forall o,
-      fe_stack_data fe <= o < fe_stack_data fe + bound_stack_data b ->
-      fe_ofs_arg <= o < fe_ofs_arg + 4 * bound_outgoing b ->
-      False.
-Proof.
-  clear. intros b fe.
-  generalize (frame_env_separated' b).
-  simpl. intuition.
-  cut (o < o). omega.
-  eapply Z.lt_le_trans.
-  apply H9. etransitivity.
-  2: apply H7.
-  etransitivity. 2: apply align_le ; try omega.
-  etransitivity. 2: apply le_add_pos; [ generalize (bound_local_pos b); omega].
-  etransitivity. 2: apply align_le ; try omega.
-  etransitivity. 2: apply size_callee_save_area_incr.
-  change fe_ofs_arg with 0.
-  rewrite Z.add_0_l.
-  apply align_le. destr; omega.
-Qed.
-
-Lemma stkdata_local_sep:
-  forall b,
-    let fe := make_env b in
-    forall o,
-      fe_stack_data fe <= o < fe_stack_data fe + bound_stack_data b ->
-      fe_ofs_local fe <= o < fe_ofs_local fe + 4 * bound_local b ->
-      False.
-Proof.
-  clear. intros b fe.
-  generalize (frame_env_separated' b).
-  simpl. intuition.
-Qed.
-
-End WITHMEM.
