backend/#Mach_old.v#
@@ -18,17 +18,17 @@
 
 Require Import Coqlib.
 Require Import Maps.
-Require Import AST.
+Require Import AST_old.
 Require Import Integers.
-Require Import Values.
-Require Import Memory.
-Require Import Globalenvs.
-Require Import Events.
-Require Import Smallstep.
-Require Import Op.
-Require Import Locations.
-Require Import Conventions.
-Require Stacklayout.
+Require Import Values_old.
+Require Import Memory_old.
+Require Import Globalenvs_old.
+Require Import Events_old.
+Require Import Smallstep_old.
+Require Import Op_old.
+Require Import Locations_old.
+Require Import Conventions_old.
+Require Import Stacklayout_old.
 
 (** * Abstract syntax *)
 
@@ -73,12 +73,14 @@ Record function: Type := mkfunction
   { fn_sig: signature;
     fn_code: code;
     fn_stacksize: Z;
-(*SACC:comments this*)(*fn_link_ofs: ptrofs;*)
-    fn_retaddr_ofs: ptrofs }.
+    (* fn_link_ofs: ptrofs; *)
+    fn_retaddr_ofs: ptrofs;
+    fn_frame_pubrange: Z * Z;
+  }.
 
-Definition fundef := AST.fundef function.
+Definition fundef := AST_old.fundef function.
 
-Definition program := AST.program fundef unit.
+Definition program := AST_old.program fundef unit.
 
 Definition funsig (fd: fundef) :=
   match fd with
@@ -118,34 +120,16 @@ value of the return address that the Asm code generated later will
 store in the reserved location.
 *)
 
+Section WITHMEMORYMODELOPS.
+Context `{memory_model_ops: Mem.MemoryModelOps}.
+
 Definition load_stack (m: mem) (sp: val) (ty: typ) (ofs: ptrofs) :=
   Mem.loadv (chunk_of_type ty) m (Val.offset_ptr sp ofs).
 
 Definition store_stack (m: mem) (sp: val) (ty: typ) (ofs: ptrofs) (v: val) :=
   Mem.storev (chunk_of_type ty) m (Val.offset_ptr sp ofs) v.
 
-(*SACC:*)
-Lemma store_stack_no_abstract:
-  forall sp ty o v m m',
-    store_stack m sp ty o v = Some m' ->
-    Mem.stack m' = Mem.stack m.
-Proof.
-  unfold store_stack, Mem.storev.
-  intros.
-  destruct (Val.offset_ptr sp o); try discriminate.
-  eapply Mem.store_stack_unchanged; eauto.
-Qed.
-
-(*SACC:
-Lemma store_stack_nextblock:
-  forall m v ty p v1 m',
-    store_stack m v ty p v1 = Some m' ->
-    Mem.nextblock m' = Mem.nextblock m.
-Proof.
-  unfold store_stack; intros.
-  destruct (Val.offset_ptr v p); simpl in *; inv H;  eauto with mem.
-Qed.
-*)
+End WITHMEMORYMODELOPS.
 
 Module RegEq.
   Definition t := mreg.
@@ -219,16 +203,6 @@ Proof.
   destruct (is_label lbl a). inv H. auto with coqlib. eauto with coqlib.
 Qed.
 
-Section STACK_WRAPPER.
-
-Variable invalidate_frame: mem -> option mem.
-
-Section RELSEM.
-
-Variable return_address_offset: function -> code -> ptrofs -> Prop.
-
-Variable ge: genv.
-
 Definition find_function_ptr
         (ge: genv) (ros: mreg + ident) (rs: regset) : option block :=
   match ros with
@@ -243,11 +217,14 @@ Definition find_function_ptr
 
 (** Extract the values of the arguments to an external call. *)
 
+Section WITHMEMORYMODELOPS2.
+Context `{memory_model_ops: Mem.MemoryModelOps}.
+
 Inductive extcall_arg (rs: regset) (m: mem) (sp: val): loc -> val -> Prop :=
   | extcall_arg_reg: forall r,
       extcall_arg rs m sp (R r) (rs r)
   | extcall_arg_stack: forall ofs ty v,
-      load_stack m sp ty (Ptrofs.repr (Stacklayout.fe_ofs_arg + 4 * ofs)) = Some v ->
+      load_stack m sp ty (Ptrofs.repr (Stacklayout_old.fe_ofs_arg + 4 * ofs)) = Some v ->
       extcall_arg rs m sp (S Outgoing ofs ty) v.
 
 Inductive extcall_arg_pair (rs: regset) (m: mem) (sp: val): rpair loc -> val -> Prop :=
@@ -263,19 +240,19 @@ Definition extcall_arguments
     (rs: regset) (m: mem) (sp: val) (sg: signature) (args: list val) : Prop :=
   list_forall2 (extcall_arg_pair rs m sp) (loc_arguments sg) args.
 
-(** Mach execution states. *)
+End WITHMEMORYMODELOPS2.
 
 (** Mach execution states. *)
 
 Inductive stackframe: Type :=
   | Stackframe:
       forall (f: block)       (**r pointer to calling function *)
-             (sp: (*SACC:*) block)        (**r stack pointer in calling function *)
+             (sp: block)        (**r stack pointer in calling function *)
              (retaddr: val)   (**r Asm return address in calling function *)
              (c: code),       (**r program point in calling function *)
       stackframe.
 
-Inductive state: Type :=
+Inductive state `{memory_model_ops: Mem.MemoryModelOps}: Type :=
   | State:
       forall (stack: list stackframe)  (**r call stack *)
              (f: block)                (**r pointer to current function *)
@@ -296,19 +273,28 @@ Inductive state: Type :=
              (m: mem),                 (**r memory state *)
       state.
 
-(*SACC: Use StackADT one instead*)(*
-Definition parent_sp (s: list stackframe) : val :=
-  match s with
-  | nil => Vnullptr
-  | Stackframe f sp ra c :: s' => sp
-  end.
-*)
+Section WITHEXTERNALCALLSOPS.
+Context `{external_calls: ExternalCalls}.
+
+Section RELSEM.
+Variables init_ra: val.
 
 Definition parent_ra (s: list stackframe) : val :=
   match s with
-  | nil => Vnullptr
+  | nil => init_ra
   | Stackframe f sp ra c :: s' => ra
   end.
+
+Variable return_address_offset: function -> code -> ptrofs -> Prop.
+
+Variable invalidate_frame: mem -> option mem.
+
+Variable ge: genv.
+
+Definition check_alloc_frame (f: frame_info) (fn: function) :=
+  0 < (frame_size f).
+
+
 
 Inductive step: state -> trace -> state -> Prop :=
   | exec_Mlabel:
@@ -329,8 +315,8 @@ Inductive step: state -> trace -> state -> Prop :=
   | exec_Mgetparam:
       forall s fb f sp ofs ty dst c rs m v rs',
       Genv.find_funct_ptr ge fb = Some (Internal f) ->
-      (*SACC: comments this*)(*load_stack m sp Tptr f.(fn_link_ofs) = Some (parent_sp s) ->*)
-      load_stack m (parent_sp ((*SACC:*)Mem.stack m)) ty ofs = Some v ->
+      (* load_stack m sp Tptr f.(fn_link_ofs) = Some (parent_sp s) -> *)
+      load_stack m (parent_sp (Mem.stack m)) ty ofs = Some v ->
       rs' = (rs # temp_for_parent_frame <- Vundef # dst <- v) ->
       step (State s fb sp (Mgetparam ofs ty dst :: c) rs m)
         E0 (State s fb sp c rs' m)
@@ -356,34 +342,33 @@ Inductive step: state -> trace -> state -> Prop :=
         E0 (State s f sp c rs' m')
   | exec_Mcall:
       forall s fb sp sig ros c rs m f f' ra,
-      find_function_ptr ge ros rs = Some f' ->
-  (*SACC:*)(exists fd, Genv.find_funct_ptr ge f' = Some fd) ->
+        find_function_ptr ge ros rs = Some f' ->
+        (exists fd, Genv.find_funct_ptr ge f' = Some fd) ->
       Genv.find_funct_ptr ge fb = Some (Internal f) ->
       return_address_offset f c ra ->
-      step (State s fb (*SACC:*)(Vptr sp Ptrofs.zero) (Mcall sig ros :: c) rs m)
+      step (State s fb (Vptr sp Ptrofs.zero) (Mcall sig ros :: c) rs m)
         E0 (Callstate (Stackframe fb sp (Vptr fb ra) c :: s)
-                       f' rs ((*SACC:*)Mem.push_new_stage m))
+                       f' rs (Mem.push_new_stage m))
   | exec_Mtailcall:
-      forall s fb stk soff sig ros c rs m f f' m' (*SACC:*)m'',
-      find_function_ptr ge ros rs = Some f' ->
-  (*SACC:*)(exists fd, Genv.find_funct_ptr ge f' = Some fd) ->
+      forall s fb stk soff sig ros c rs m f f' m' m'',
+        find_function_ptr ge ros rs = Some f' ->
+        (exists fd, Genv.find_funct_ptr ge f' = Some fd) ->
       Genv.find_funct_ptr ge fb = Some (Internal f) ->
-  (*SACC:comments this*)(*load_stack m (Vptr stk soff) Tptr f.(fn_link_ofs) = Some (parent_sp s) ->
-      load_stack m (Vptr stk soff) Tptr f.(fn_retaddr_ofs) = Some (parent_ra s) ->
-      Mem.free m stk 0 f.(fn_stacksize) = Some m' ->*)
-  (*SACC:*)Mem.loadbytesv Mptr m (Val.offset_ptr (Vptr stk soff) f.(fn_retaddr_ofs)) = Some (parent_ra s) ->
-  (*SACC:*)Mem.free m stk (Ptrofs.unsigned soff) (Ptrofs.unsigned soff + f.(fn_stacksize)) = Some m' ->
-  (*SACC:*)Mem.tailcall_stage m' = Some m'' ->
+      (* load_stack m (Vptr stk soff) Tptr f.(fn_link_ofs) = Some (parent_sp s) -> *)
+      Mem.loadbytesv Mptr m (Val.offset_ptr (Vptr stk soff) f.(fn_retaddr_ofs)) = Some (parent_ra s) ->
+      Mem.free m stk (Ptrofs.unsigned soff) (Ptrofs.unsigned soff + f.(fn_stacksize)) = Some m' ->
+      Mem.tailcall_stage m' = Some m'' ->
       step (State s fb (Vptr stk soff) (Mtailcall sig ros :: c) rs m)
-        E0 (Callstate s f' rs (*SACC:*)m'')
+        E0 (Callstate s f' rs m'')
   | exec_Mbuiltin:
-      forall s f sp rs m ef args res b vargs t vres rs' m' (*SACC:*)m'',
+      forall s f sp rs m ef args res b vargs t vres rs' m' m'',
       eval_builtin_args ge rs sp m args vargs ->
-      external_call ef ge vargs ((*SACC:*)Mem.push_new_stage m) t vres m' ->
-  (*SACC:*)Mem.unrecord_stack_block m' = Some m'' ->
+      external_call ef ge vargs (Mem.push_new_stage m) t vres m' ->
+      Mem.unrecord_stack_block m' = Some m'' ->                                          
       rs' = set_res res vres (undef_regs (destroyed_by_builtin ef) rs) ->
+      forall BUILTIN_ENABLED : builtin_enabled ef,
       step (State s f sp (Mbuiltin ef args res :: b) rs m)
-         t (State s f sp b rs' (*SACC:*)m'')
+         t (State s f sp b rs' m'')
   | exec_Mgoto:
       forall s fb f sp lbl c rs m c',
       Genv.find_funct_ptr ge fb = Some (Internal f) ->
@@ -414,51 +399,38 @@ Inductive step: state -> trace -> state -> Prop :=
       step (State s fb sp (Mjumptable arg tbl :: c) rs m)
         E0 (State s fb sp c' rs' m)
   | exec_Mreturn:
-      forall s fb stk soff c rs m f m' (*SACC:*)m'',
+      forall s fb stk soff c rs m f m' m'',
       Genv.find_funct_ptr ge fb = Some (Internal f) ->
-      (*SACC:comments this*)(*
-      load_stack m (Vptr stk soff) Tptr f.(fn_link_ofs) = Some (parent_sp s) ->
-      load_stack m (Vptr stk soff) Tptr f.(fn_retaddr_ofs) = Some (parent_ra s) ->
-      Mem.free m stk 0 f.(fn_stacksize) = Some m' ->*)
-  (*SACC:*)Mem.loadbytesv Mptr m (Val.offset_ptr (Vptr stk soff) f.(fn_retaddr_ofs)) = Some (parent_ra s) ->
-  (*SACC:*)Mem.free m stk (Ptrofs.unsigned soff) (Ptrofs.unsigned soff + f.(fn_stacksize)) = Some m' ->
-  (*SACC:*)invalidate_frame m' = Some m'' ->
+      Mem.loadbytesv Mptr m (Val.offset_ptr (Vptr stk soff) f.(fn_retaddr_ofs)) = Some (parent_ra s) ->
+      Mem.free m stk (Ptrofs.unsigned soff) (Ptrofs.unsigned soff + f.(fn_stacksize)) = Some m' ->
+      invalidate_frame m' = Some m'' ->
       step (State s fb (Vptr stk soff) (Mreturn :: c) rs m)
-        E0 (Returnstate s rs (*SACC:*)m'')
+        E0 (Returnstate s rs m'')
   | exec_function_internal:
-      forall s fb rs m f m1 m2 m3 stk rs',
+      forall s fb rs m f m1 m1_ m3 stk rs' fi,
       Genv.find_funct_ptr ge fb = Some (Internal f) ->
+      frame_info_of_size_and_pubrange (fn_stacksize f) (fn_frame_pubrange f) = Some fi ->
       Mem.alloc m 0 f.(fn_stacksize) = (m1, stk) ->
       let sp := Vptr stk Ptrofs.zero in
-      (*SACC:comments this*)(*
-      store_stack m1 sp Tptr f.(fn_link_ofs) (parent_sp s) = Some m2 ->*)
-      store_stack m1 sp Tptr f.(fn_retaddr_ofs) (parent_ra s) = Some m2 ->
-  (*SACC:*)Mem.record_stack_blocks m2 (make_singleton_frame_adt stk (fn_stacksize f)  (fn_stacksize f)) = Some m3 ->
+      (* store_stack m1 sp Tptr f.(fn_link_ofs) (parent_sp s) = Some m2 -> *)
+      store_stack m1 sp Tptr f.(fn_retaddr_ofs) (parent_ra s) = Some m3 ->
+      Mem.record_stack_blocks m3 (make_singleton_frame_adt' stk fi (fn_stacksize f)) = Some m1_ ->
       rs' = undef_regs destroyed_at_function_entry rs ->
       step (Callstate s fb rs m)
-        E0 (State s fb sp f.(fn_code) rs' m3)
+        E0 (State s fb sp f.(fn_code) rs' m1_)
   | exec_function_external:
       forall s fb rs m t rs' ef args res m',
       Genv.find_funct_ptr ge fb = Some (External ef) ->
       extcall_arguments rs m (parent_sp (Mem.stack m)) (ef_sig ef) args ->
       external_call ef ge args m t res m' ->
-      rs' = set_pair (loc_result (ef_sig ef)) res rs (*SACC:(undef_regs destroyed_at_call rs)*) ->
+      rs' = set_pair (loc_result (ef_sig ef)) res (undef_regs destroyed_at_call rs) ->
       step (Callstate s fb rs m)
          t (Returnstate s rs' m')
   | exec_return:
-      forall s f sp ra c rs m (*SACC:*)m',
-  (*SACC:*)Mem.unrecord_stack_block m = Some m' ->
+      forall s f sp ra c rs m m',
+        Mem.unrecord_stack_block m = Some m' ->
       step (Returnstate (Stackframe f sp ra c :: s) rs m)
         E0 (State s f (Vptr sp Ptrofs.zero) c rs m').
-
-(*=============================SACC:=============================*)
-Section STACK_INVARIANTS.
-
-Definition block_prop P v :=
-  match v with
-    Vptr b o => P b
-  | _ => True
-  end.
 
 Inductive callstack_function_defined : list stackframe -> Prop :=
 | cfd_empty:
@@ -485,8 +457,8 @@ Inductive init_sp_stackinfo : stack -> Prop :=
     fr tf s
     (PRIV: single_block_prop
              (fun b fi =>
-                forall o, Stacklayout.fe_ofs_arg <= o < 4 * size_arguments init_sg ->
-                     Ptrofs.unsigned (Ptrofs.repr (Stacklayout.fe_ofs_arg + o)) = Stacklayout.fe_ofs_arg + o)
+                forall o, fe_ofs_arg <= o < 4 * size_arguments init_sg ->
+                     frame_private fi o /\ Ptrofs.unsigned (Ptrofs.repr (fe_ofs_arg + o)) = fe_ofs_arg + o)
              (frame_adt_blocks fr)):
     init_sp_stackinfo ((Some fr,tf)::s).
 
@@ -497,6 +469,20 @@ Inductive list_prefix : list (option (block * frame_info)) -> stack -> Prop :=
                    (FSIZE: frame_adt_size f = frame_size bi)
                    (BLOCKS: frame_adt_blocks f = (sp,bi)::nil):
     list_prefix (Some (sp,bi) :: lsp) ( (Some f , r) :: s).
+
+Definition stack_blocks_of_callstack (l : list stackframe) : list (option (block * frame_info)) :=
+  map (fun x =>
+         match x with
+           Stackframe fb sp _ _ =>
+           match Genv.find_funct_ptr ge fb with
+             Some (Internal f) =>
+             match frame_info_of_size_and_pubrange (fn_stacksize f) (fn_frame_pubrange f) with
+             | Some fi => Some (sp, fi)
+             | None => None
+             end
+           | _ => None
+           end
+         end) l.
 
 Inductive has_code: state -> Prop :=
 | has_code_intro fb f cs sp c rs m
@@ -522,6 +508,7 @@ Proof.
   apply IHc in H. destruct H as (l & CODE); rewrite CODE.
   exists (a::l); simpl. reflexivity.
 Qed.
+
 
 Lemma has_code_step:
   forall s1 t s2,
@@ -565,22 +552,12 @@ Proof.
     eexists (l ++ _ :: nil); simpl; rewrite app_ass; reflexivity.
 Qed.
 
-Definition stack_blocks_of_callstack (l : list stackframe) : list (option (block * frame_info)) :=
-  map (fun x =>
-         match x with
-           Stackframe fb sp _ _ =>
-           match Genv.find_funct_ptr ge fb with
-             Some (Internal f) =>
-              Some (sp, default_frame_info (fn_stacksize f))
-           | _ => None
-           end
-         end) l.
-
 Inductive call_stack_consistency: state -> Prop :=
 | call_stack_consistency_intro:
-    forall c cs' fb sp' rs m' tf
+    forall c cs' fb sp' rs m' tf fi
       (FIND: Genv.find_funct_ptr ge fb = Some (Internal tf))
-      (CallStackConsistency: list_prefix ((Some (sp', default_frame_info (fn_stacksize tf)))::stack_blocks_of_callstack cs') (Mem.stack m'))
+      (FRAME: frame_info_of_size_and_pubrange (fn_stacksize tf) (fn_frame_pubrange tf) = Some fi)
+      (CallStackConsistency: list_prefix ((Some (sp', fi))::stack_blocks_of_callstack cs') (Mem.stack m'))
     ,
       call_stack_consistency (State cs' fb (Vptr sp' Ptrofs.zero) c rs m')
 | call_stack_consistency_call:
@@ -594,6 +571,16 @@ Inductive call_stack_consistency: state -> Prop :=
       (TTNP: Mem.top_frame_no_perm m'),
       call_stack_consistency (Returnstate cs' rs m').
 
+Lemma store_stack_no_abstract:
+  forall sp ty o v,
+    Mem.stack_unchanged (fun m m' => store_stack m sp ty o v = Some m').
+Proof.
+  unfold store_stack, Mem.storev.
+  red; simpl; intros.
+  destruct (Val.offset_ptr sp o); try discriminate.
+  eapply Mem.store_no_abstract; eauto.
+Qed.
+
 Hypothesis invalidate_frame_tl_stack:
   forall m1 m2,
     invalidate_frame m1 = Some m2 ->
@@ -604,6 +591,7 @@ Hypothesis invalidate_frame_top_no_perm:
     invalidate_frame m1 = Some m2 ->
     Mem.top_frame_no_perm m1 ->
     Mem.top_frame_no_perm m2.
+
 
 Ltac same_hyps :=
   repeat match goal with
@@ -621,10 +609,10 @@ Proof.
   destruct 1; simpl; intros SIZE HC CSC; inv HC; inv CSC;
     same_hyps;
     try now (econstructor; eauto).
-  - econstructor; eauto. erewrite store_stack_no_abstract; eauto. 
-  - econstructor; eauto. destruct a; simpl in *; try discriminate. erewrite Mem.store_stack_unchanged; eauto.
+  - econstructor; eauto. erewrite store_stack_no_abstract; eauto.
+  - econstructor; eauto. destruct a; simpl in *; try discriminate. erewrite Mem.store_no_abstract; eauto.
   - econstructor. rewrite_stack_blocks. simpl. 
-    rewrite H1. auto.
+    rewrite H1. rewrite FRAME. auto.
     red. rewrite_stack_blocks. constructor. reflexivity.
   - econstructor. repeat rewrite_stack_blocks. simpl. intro EQ; rewrite EQ in CallStackConsistency.
     inv CallStackConsistency; simpl; auto.
@@ -636,35 +624,242 @@ Proof.
     eapply invalidate_frame_top_no_perm; eauto.
     inv CallStackConsistency.
     eapply Mem.free_top_tframe_no_perm; eauto.
+    unfold frame_info_of_size_and_pubrange in FRAME; repeat destr_in FRAME. simpl.
+    rewrite Ptrofs.unsigned_zero.
+    simpl. rewrite Z.max_r. auto. omega.
   - econstructor; eauto; repeat rewrite_stack_blocks; simpl; eauto.
     repeat econstructor; eauto.
-    Check store_stack_no_abstract.
-    rewrite (store_stack_no_abstract _ _ _ _ _ _ H1) in EQ1.
+    rewrite store_stack_no_abstract in EQ1 by eauto.
     revert EQ1; rewrite_stack_blocks. intro. rewrite EQ1 in CallStackConsistency. simpl in *.
     auto.
+    simpl.
+    unfold frame_info_of_size_and_pubrange in H0; repeat destr_in H0. simpl.
+    apply Z.max_r. omega.
   - econstructor; eauto; repeat rewrite_stack_blocks; simpl; eauto.
     red; rewrite_stack_blocks.
     inv TTNP.
     constructor. unfold in_frames; rewrite H3; easy.
   - inv CFD. simpl in CallStackConsistency.
-    rewrite FINDF in CallStackConsistency.
-    exploit SIZE; eauto. intros. 
-    econstructor; eauto.
-    repeat rewrite_stack_blocks; simpl; eauto.
+    rewrite FINDF in CallStackConsistency. destr_in CallStackConsistency. eauto.
+    econstructor; eauto; repeat rewrite_stack_blocks; simpl; eauto.
+    unfold frame_info_of_size_and_pubrange in Heqo. repeat destr_in Heqo.
+    exploit SIZE; eauto. omega.
 Qed.
 
-End STACK_INVARIANTS.
+Definition mem_state (s: state) : mem :=
+  match s with
+    State _ _ _ _ _ m
+  | Callstate _ _ _ m
+  | Returnstate _ _ m => m
+  end.
+
+Lemma list_prefix_in_init_stk:
+  forall cs s,
+    list_prefix cs s ->
+    forall b,
+      in_stack init_stk b ->
+      in_stack s b.
+Proof.
+  induction 1; intros. subst; auto.
+  rewrite in_stack_cons; right; eauto.
+Qed.
+
+Lemma list_prefix_stack_top_not_init_stk':
+  forall b b' f fr cs s,
+    nodup (fr::s) ->
+    list_prefix (Some (b',f)::cs) (fr::s) ->
+    in_frames fr b ->
+    get_frame_info init_stk b = None.
+Proof.
+  intros.
+  destruct (get_frame_info init_stk b) eqn:GFI; auto.
+  apply get_frame_info_in_stack in GFI. exfalso.
+  inv H0.
+  inv H.
+  eapply H4. eauto.
+  eapply list_prefix_in_init_stk. eauto. auto.
+Qed.
+
+Lemma list_prefix_stack_top_not_init_stk:
+  forall b b' f cs s,
+    nodup s ->
+    list_prefix (Some (b',f)::cs) s ->
+    is_stack_top s b ->
+    get_frame_info init_stk b = None.
+Proof.
+  intros.
+  inv H0. red in H1. simpl in H1.
+  eapply list_prefix_stack_top_not_init_stk'. eauto. constructor; eauto. auto.
+Qed.
+
+Lemma list_prefix_not_in_init_stk:
+  forall b f cs s,
+    nodup s ->
+    list_prefix (Some (b, f)::cs) s ->
+    get_frame_info init_stk b = None.
+Proof.
+  intros.
+  destruct (get_frame_info init_stk b) eqn:GFI; auto.
+  apply get_frame_info_in_stack in GFI. exfalso.
+  inv H0.
+  inv H.
+  eapply H3. rewrite in_frames_cons. eexists; split. reflexivity. 
+  eapply in_frame'_in_frame. red. rewrite BLOCKS. left; reflexivity.
+  eapply list_prefix_in_init_stk. eauto. auto.
+Qed.
+
+Lemma public_stack_access_init_stk:
+  forall cs s b lo hi
+         (LP: list_prefix cs s)
+         (ND: nodup s)
+         (PSA: public_stack_access s b lo hi),
+    public_stack_access init_stk b lo hi.
+Proof.
+  induction 1; simpl; subst; auto.
+  intros.
+  apply IHLP. inv ND; auto.
+  red. red in PSA. destr.
+  edestruct (get_assoc_spec _ _ _ Heqo) as (fr & tf & INblocks & INtf & INs).
+  erewrite get_assoc_stack_lnr in PSA. eauto. eauto. eauto. eauto. eauto. right; auto.
+Qed.
+
+Lemma public_stack_access_init_stk':
+  forall cs s b lo hi
+         (LP: list_prefix cs s)
+         f
+         (ND: nodup (f::s))
+         (PSA: public_stack_access (f::s) b lo hi),
+    public_stack_access init_stk b lo hi.
+Proof.
+  induction 1; simpl; subst; auto.
+  - unfold public_stack_access. simpl.
+    intros. destr.
+    destr_in PSA. destr_in Heqo0.
+    inv ND.
+    exfalso; eapply H2; eauto. eapply get_frame_info_in_stack; eauto.
+    inv Heqo0; auto.
+    repeat destr_in Heqo0.
+    inv ND.
+    exfalso; eapply H3; eauto. eapply get_frame_info_in_stack; eauto.
+  - intros.
+    eapply IHLP. inv ND; eauto.
+    red. red in PSA. destr.
+    edestruct (get_assoc_spec _ _ _ Heqo) as (fr & tf & INblocks & INtf & INs).
+    erewrite get_assoc_stack_lnr in PSA. eauto. eauto. eauto.
+    eauto. eauto. right; auto.
+Qed.
+
+
+Hypothesis invalidate_frame_unchanged_on:
+  forall m1 m2 P,
+    invalidate_frame m1 = Some m2 ->
+    Mem.unchanged_on P m1 m2.
+
+Lemma csc_unchanged_stack:
+  forall s t s',
+    step s t s' ->
+    call_stack_consistency s ->
+    Mem.unchanged_on
+      (fun b o => ~ stack_access init_stk b o (o+1))
+      (mem_state s) (mem_state s').
+Proof.
+  intros s t s' STEP CSC. inv STEP; inv CSC; simpl; try apply Mem.unchanged_on_refl.
+  - unfold store_stack in H. simpl in H.
+    eapply Mem.store_unchanged_on; eauto.
+    intros i RNG PSA; apply PSA; clear PSA. red.
+    right. red. erewrite list_prefix_not_in_init_stk; eauto. apply Mem.stack_norepet.
+  - unfold Mem.storev in H0. destr_in H0.
+    eapply Mem.store_unchanged_on; eauto.
+    intros i0 RNG PSA; apply PSA; clear PSA.
+    edestruct Mem.store_valid_access_3 as (A & B & C). eauto. trim C. constructor.
+    destruct C as [IST|NPSA].
+    right. red; erewrite list_prefix_stack_top_not_init_stk; eauto. apply Mem.stack_norepet.
+    right. eapply public_stack_access_inside.
+    eapply public_stack_access_init_stk; eauto. apply Mem.stack_norepet.
+    omega. omega.
+  - apply Mem.strong_unchanged_on_weak. apply Mem.push_new_stage_unchanged_on.
+  - eapply Mem.unchanged_on_trans. eapply Mem.free_unchanged_on; eauto.
+    intros i RNG PSA; apply PSA; clear PSA. right; red.
+    erewrite list_prefix_not_in_init_stk; eauto. apply Mem.stack_norepet.
+    eapply Mem.strong_unchanged_on_weak, Mem.tailcall_stage_unchanged_on; eauto.
+  - exploit ec_unchanged_on_private_stack. apply external_call_spec. eauto.
+    intros.
+    eapply Mem.unchanged_on_trans.
+    apply Mem.strong_unchanged_on_weak. eapply Mem.push_new_stage_unchanged_on.
+    eapply Mem.unchanged_on_trans.
+    eapply Mem.unchanged_on_implies. apply H2.
+    simpl.
+    intros b0 ofs NPSA VB PSA.
+    apply NPSA.
+    assert (PSA': stack_access (Mem.stack m) b0 ofs (ofs + 1)).
+    {
+      red in PSA. revert PSA. red. rewrite_stack_blocks. unfold is_stack_top. simpl.  unfold public_stack_access. simpl. auto.
+      intros [[]|P]. right. auto.
+    } clear PSA.
+    destruct PSA'.
+    right; red. erewrite list_prefix_stack_top_not_init_stk; eauto. apply Mem.stack_norepet.
+    right.
+    eapply public_stack_access_init_stk. 4: eauto. eauto. apply Mem.stack_norepet.
+    auto.
+    apply Mem.strong_unchanged_on_weak. eapply Mem.unrecord_stack_block_unchanged_on. eauto.
+  - eapply Mem.unchanged_on_trans. eapply Mem.free_unchanged_on; eauto.
+    intros i RNG PSA; apply PSA; clear PSA. right; red.
+    erewrite list_prefix_not_in_init_stk; eauto. apply Mem.stack_norepet.
+    eapply invalidate_frame_unchanged_on; eauto.
+  - eapply Mem.unchanged_on_trans.
+    eapply Mem.alloc_unchanged_on; eauto.
+    unfold store_stack in H2. subst. simpl in H2.
+    eapply Mem.unchanged_on_trans.
+    eapply Mem.store_unchanged_on. eauto.
+    intros i0 RNG PSA; apply PSA; clear PSA.
+    right; red. destr.
+    apply get_frame_info_in_stack in Heqo. exfalso.
+    eapply list_prefix_in_init_stk in Heqo; eauto.
+    apply in_stack_tl in Heqo. apply Mem.in_frames_valid in Heqo.
+    eapply Mem.fresh_block_alloc; eauto.
+    apply Mem.strong_unchanged_on_weak. eapply Mem.record_stack_block_unchanged_on. eauto.
+  - exploit ec_unchanged_on_private_stack. apply external_call_spec. eauto.
+    intros.
+    eapply Mem.unchanged_on_implies. apply H2.
+    simpl.
+    intros b0 ofs NPSA VB PSA.
+    apply NPSA. inv TTNP. rewrite <- H3 in CallStackConsistency. simpl in CallStackConsistency.
+    destruct PSA.
+    right; red.
+    destr. eapply get_frame_info_in_stack in Heqo.
+    eapply list_prefix_in_init_stk in Heqo; eauto.
+    exploit Mem.stack_norepet. rewrite <- H3. intro ND. inv ND. edestruct H9; eauto.
+    rewrite <- H3 in H5. red in H5. eauto.
+    right.
+    rewrite <- H3 in *.
+    eapply public_stack_access_init_stk' . 3: eauto. eauto.
+    rewrite H3; apply Mem.stack_norepet.
+  - apply Mem.strong_unchanged_on_weak. eapply Mem.unrecord_stack_block_unchanged_on. eauto.
+Qed.
+
+Definition block_prop P v :=
+  match v with
+    Vptr b o => P b
+  | _ => True
+  end.
+
+Lemma store_stack_nextblock:
+  forall m v ty p v1 m',
+    store_stack m v ty p v1 = Some m' ->
+    Mem.nextblock m' = Mem.nextblock m.
+Proof.
+  unfold store_stack; intros.
+  destruct (Val.offset_ptr v p); simpl in *; inv H;  eauto with mem.
+Qed.
 
 End RELSEM.
 
-End STACK_WRAPPER.
-
 Inductive initial_state (p: program): state -> Prop :=
-  | initial_state_intro: forall fb m0 (*SACC:*)m2,
+  | initial_state_intro: forall fb m0 m2,
       let ge := Genv.globalenv p in
       Genv.init_mem p = Some m0 ->
       Genv.find_symbol ge p.(prog_main) = Some fb ->
-  (*SACC:*)Mem.record_init_sp m0 = Some m2 ->
+      Mem.record_init_sp m0 = Some m2 ->
       initial_state p (Callstate nil fb (Regmap.init Vundef) (Mem.push_new_stage m2)).
 
 Inductive final_state: state -> int -> Prop :=
@@ -673,7 +868,6 @@ Inductive final_state: state -> int -> Prop :=
       rs r = Vint retcode ->
       final_state (Returnstate nil rs m) retcode.
 
-(*==========================SACC: invalidate_frame interface==========================*)
 Definition invalidate_frame1 (m: mem) := Some m.
 
 Lemma invalidate_frame1_tl_stack:
@@ -691,6 +885,14 @@ Lemma invalidate_frame1_top_no_perm:
     Mem.top_frame_no_perm m2.
 Proof.
   unfold invalidate_frame1; intros m1 m2 EQ; inv EQ; auto.
+Qed.
+
+Lemma invalidate_frame1_unchanged_on:
+  forall m1 m2 P,
+    invalidate_frame1 m1 = Some m2 ->
+    Mem.unchanged_on P m1 m2.
+Proof.
+  unfold invalidate_frame1; intros m1 m2 P EQ; inv EQ; eapply Mem.unchanged_on_refl.
 Qed.
 
 Definition invalidate_frame2 (m: mem) := Mem.tailcall_stage m.
@@ -714,10 +916,19 @@ Proof.
   constructor; unfold in_frames; simpl. rewrite H0; easy.
 Qed.
 
-(*==========================================================================================*)
+Lemma invalidate_frame2_unchanged_on:
+  forall m1 m2 P,
+    invalidate_frame2 m1 = Some m2 ->
+    Mem.unchanged_on P m1 m2.
+Proof.
+  unfold invalidate_frame2; intros m1 m2 P EQ.
+  eapply Mem.strong_unchanged_on_weak, Mem.tailcall_stage_unchanged_on; eauto.
+Qed.
 
 Definition semantics1 (rao: function -> code -> ptrofs -> Prop) (p: program) :=
-  Semantics (step invalidate_frame1 rao) (initial_state p) final_state (Genv.globalenv p).
+  Semantics (step Vnullptr rao invalidate_frame1) (initial_state p) final_state (Genv.globalenv p).
 
 Definition semantics2 (rao: function -> code -> ptrofs -> Prop) (p: program) :=
-  Semantics (step invalidate_frame2 rao) (initial_state p) final_state (Genv.globalenv p).
+  Semantics (step Vnullptr rao invalidate_frame2) (initial_state p) final_state (Genv.globalenv p).
+
+End WITHEXTERNALCALLSOPS.
